Moved termination semantics to a dedicated file.  Started bringing the Annotated syntax into line with the Surface syntax.

Total/Stlc/Lang/Annotated/Grammar.lean
@@ -1,5 +1,7 @@
 import Total.Core
 
+set_option autoImplicit false
+
 namespace Total.Stlc.Lang.Annotated
   inductive Ty: Type where
     | bool: Ty
@@ -23,17 +25,17 @@ namespace Total.Stlc.Lang.Annotated
     | gt:  PrimOp 2 (.cons .nat (.nil .nat)) .bool
     | gte: PrimOp 2 (.cons .nat (.nil .nat)) .bool
 
-  inductive Term (ρ: Ty → Type): Ty → Type where
-    | bool (b: Bool): Term ρ .bool
-    | nat (n: Nat): Term ρ .nat
-    | primOp {α: Nat} {δ: Domain Ty α} {τ: Ty} (op: PrimOp α δ τ): Term ρ (.fn δ τ)
-    | cond {τ: Ty} (c: Term ρ .bool) (t f: Term ρ τ): Term ρ τ
-    -- | var {τ: Ty} (id: Ident): Term ρ τ
-    -- | bind {τ σ: Ty} (id: Ident) (expr: Term ρ τ) (scope: Term ρ σ): Term ρ σ
-    -- | abs {α: Nat} {δ: Domain Ty α} {τ: Ty} (formals: Formals Ident Ty α δ) (body: Term ρ τ): Term ρ (.fn δ τ)
-    -- | app {α: Nat} {δ: Domain Ty α} {τ: Ty} (fn: Term ρ (.fn δ τ)) (args: Args Ty (Term ρ) α δ): Term ρ τ
+  inductive Term: Ty → Type where
+    | bool (b: Bool): Term .bool
+    | nat (n: Nat): Term .nat
+    | primOp {α: Nat} {δ: Domain Ty α} {τ: Ty} (op: PrimOp α δ τ) (operands: Args Ty (Term) α δ): Term (.fn δ τ)
+    | cond {τ: Ty} (c: Term .bool) (t f: Term τ): Term τ
+    -- | var {τ: Ty} (id: Ident): Term τ
+    -- | bind {τ σ: Ty} (id: Ident) (expr: Term τ) (scope: Term σ): Term σ
+    -- | abs {α: Nat} {δ: Domain Ty α} {τ: Ty} (formals: Params Ident Ty α δ) (body: Term τ): Term (.fn δ τ)
+    -- | app {α: Nat} {δ: Domain Ty α} {τ: Ty} (fn: Term (.fn δ τ)) (args: Args Ty (Term) α δ): Term τ
 
-  inductive Top (ρ: Ty → Type): Ty → Type where
-    -- | val (ι: Ident) (τ: Ty) (ε: Term ρ τ): Top ρ τ
-    -- | defn {α: Nat} {π: Params Ty α} {τ: Ty} (ι: Ident) (params: Formals Ident Ty α π) (body: Term ρ τ): Top ρ τ
+  inductive Top: Ty → Type where
+    -- | val (ι: Ident) (τ: Ty) (ε: Term τ): Top τ
+    -- | defn {α: Nat} {π: Params Ty α} {τ: Ty} (ι: Ident) (params: Params Ident Ty α π) (body: Term τ): Top τ
 end Total.Stlc.Lang.Annotated
