Total/Stlc/Lang/Annotated/Semantics.lean
@@ -4,87 +4,28 @@ import Total.Relation
 import Total.Stlc.Lang.Annotated.Grammar
 import Total.Stlc.Lang.Annotated.Syntax
 
+set_option autoImplicit false
+
 namespace Total.Stlc.Lang.Annotated
   namespace PrimOp
-    inductive Eval₁ (ρ: Ty → Type): (α: Nat) → (π: Domain Ty α) → (τ: Ty) → PrimOp α π τ → Term ρ τ → Prop where
+    inductive Eval₁: (α: Nat) → (π: Domain Ty α) → (τ: Ty) → PrimOp α π τ → Term τ → Prop where
   end PrimOp
 
   namespace Term
-    inductive IsValue (ρ: Ty → Type): (τ: Ty) → Term ρ τ → Prop where
-      | bool (b: Bool): IsValue ρ .bool (.bool b)
-      | nat (n: Nat): IsValue ρ .nat (.nat n)
-      -- | var (id: Ident): IsValue ρ τ (.var id)
-      -- | abs {α: Nat} {π: Params Ty α} {τ: Ty} (formals: Formals Ident Ty α π) (body: Term ρ τ): IsValue ρ (.fn π τ) (.abs formals body)
+    inductive IsValue: (τ: Ty) → Term τ → Prop where
+      | bool (b: Bool): IsValue .bool (.bool b)
+      | nat  (n: Nat):  IsValue .nat (.nat n)
+      -- | var (id: Ident): IsValue τ (.var id)
+      -- | abs {α: Nat} {π: Params Ty α} {τ: Ty} (formals: Params Ident Ty α π) (body: Term τ): IsValue (.fn π τ) (.abs formals body)
 
-    inductive Eval₁ (ρ: Ty → Type) (τ: Ty): Term ρ τ → Term ρ τ → Prop where
-    def Eval (ρ: Ty → Type) (τ: Ty) := RTC (Eval₁ ρ τ)
+    inductive Eval₁ (τ: Ty): Term τ → Term τ → Prop where
+
+    def Eval (τ: Ty) := RTC (Eval₁ τ)
   end Term
 
   namespace Top
-    inductive IsValue (ρ: Ty → Type) (τ: Ty): Top ρ τ → Prop where
-    inductive Eval₁ (ρ: Ty → Type) (τ: Ty): Top ρ τ → Top ρ τ → Prop where
-    def Eval (ρ: Ty → Type) (τ: Ty) := RTC (Eval₁ ρ τ)
-  end Top
-
-  namespace PrimOp
-    @[reducible]
-    def Halts {ρ: Ty → Type} (τ: Ty) (p: PrimOp) (t₁: Term ρ τ): Prop := ∃ t₂: Term ρ τ, Eval₁ p t₁ t₂ ∧ Term.IsValue t₂
-
-    @[reducible]
-    def Total {ρ: Ty → Type} (τ₁ τ₂: Ty) (op: UnOp) (t: Term ρ): Prop :=
-      (HasType op τ₁ τ₂) ∧ (Halts op t) ∧ True
-
-    namespace Total
-      theorem halts {τ₁ τ₂: Ty} {op: UnOp} {t: Term}: Total τ₁ τ₂ op t → Halts op t
-        | ⟨_, hh, _⟩ => hh
-    end Total
-  end PrimOp
-
-  namespace Term
-    @[reducible]
-    def Halts {ρ: Ty → Type} {τ: Ty} (t₁: Term ρ τ): Prop := ∃ t₂: Term ρ τ, Eval ρ τ t₁ t₂ ∧ IsValue ρ τ t₂
-
-    @[reducible]
-    def Total {ρ: Ty → Type} (τ: Ty) (t: Term ρ τ): Prop :=
-      (Halts t) ∧ (
-        match τ with
-          | .bool => True
-          | .nat  => True
-          | .fn _ _ => sorry
-      )
-
-    namespace IsValue
-      theorem halts {ρ: Ty → Type} {τ: Ty} {t: Term ρ τ}: IsValue ρ τ t → Halts t
-        | .bool _ => ⟨_, .refl, .bool _⟩
-        | .nat  _ => ⟨_, .refl, .nat  _⟩
-    end IsValue
-
-    namespace Total
-      theorem halts {ρ: Ty → Type} {τ: Ty}: {t: Term ρ τ} → Total τ t → Halts t
-        | .bool _, _ => IsValue.halts (.bool _)
-        | .nat _,  _ => IsValue.halts (.nat  _)
-
-        | .primOp _, _ => sorry
-
-        | .cond _ _ _,  ⟨_, ⟨_, he, hv⟩, _⟩ => ⟨_, he, hv⟩
-    end Total
-  end Term
-
-  namespace Top
-    @[reducible]
-    def Halts {ρ: Ty → Type} {τ: Ty} (t₁: Top ρ τ): Prop := ∃ t₂: Top ρ τ, Eval ρ τ t₁ t₂ ∧ IsValue ρ τ t₂
-
-    @[reducible]
-    def Total {ρ: Ty → Type} {τ: Ty}: Ty → Top ρ τ → Prop
-      | .bool, t => nomatch t
-
-    namespace IsValue
-      theorem halts {ρ: Ty → Type} {τ: Ty} {t: Top ρ τ}: IsValue ρ τ t → Halts t := nomatch t
-    end IsValue
-
-    namespace Total
-      theorem halts {ρ: Ty → Type} {τ: Ty} {t: Top ρ τ}: Top ρ τ → Halts t
-        | t => nomatch t
-    end Total
+    inductive IsValue (τ: Ty): Top τ → Prop where
+    inductive Eval₁ (τ: Ty): Top τ → Top τ → Prop where
+    def Eval (τ: Ty) := RTC (Eval₁ τ)
   end Top
 end Total.Stlc.Lang.Annotated
