Total/Stlc/Lang/Annotated/Termination.lean
@@ -1,0 +1,72 @@
+import Total.Core
+import Total.Relation
+
+import Total.Stlc.Lang.Annotated.Grammar
+import Total.Stlc.Lang.Annotated.Syntax
+import Total.Stlc.Lang.Annotated.Semantics
+
+set_option autoImplicit false
+
+namespace Total.Stlc.Lang.Annotated
+  namespace PrimOp
+    @[reducible]
+    def Halts (τ: Ty) (p: PrimOp) (t₁: Term τ): Prop := ∃ t₂: Term τ, Eval₁ t₁ t₂ ∧ Term.IsValue t₂
+
+    @[reducible]
+    def Total (τ₁ τ₂: Ty) (op: UnOp) (t: Term): Prop :=
+      (HasType op τ₁ τ₂) ∧ (Halts op t) ∧ True
+
+    namespace Total
+      theorem halts {τ₁ τ₂: Ty} {op: UnOp} {t: Term}: Total τ₁ τ₂ op t → Halts op t
+        | ⟨_, hh, _⟩ => hh
+    end Total
+  end PrimOp
+
+  namespace Term
+    @[reducible]
+    def Halts {τ: Ty} (t₁: Term τ): Prop := ∃ t₂: Term τ, Eval τ t₁ t₂ ∧ IsValue τ t₂
+
+    @[reducible]
+    def Total (τ: Ty) (t: Term τ): Prop :=
+      (Halts t) ∧ (
+        match τ with
+          | .bool => True
+          | .nat  => True
+          | .fn _ _ => sorry
+      )
+
+    namespace IsValue
+      theorem halts {τ: Ty} {t: Term τ}: IsValue τ t → Halts t
+        | .bool _ => ⟨_, .refl, .bool _⟩
+        | .nat  _ => ⟨_, .refl, .nat  _⟩
+    end IsValue
+
+    namespace Total
+      theorem halts {τ: Ty}: {t: Term τ} → Total τ t → Halts t
+        | .bool _, _ => IsValue.halts (.bool _)
+        | .nat _,  _ => IsValue.halts (.nat  _)
+
+        | .primOp _, _ => sorry
+
+        | .cond _ _ _,  ⟨_, ⟨_, he, hv⟩, _⟩ => ⟨_, he, hv⟩
+    end Total
+  end Term
+
+  namespace Top
+    @[reducible]
+    def Halts {τ: Ty} (t₁: Top τ): Prop := ∃ t₂: Top τ, Eval τ t₁ t₂ ∧ IsValue τ t₂
+
+    @[reducible]
+    def Total {τ: Ty}: Ty → Top τ → Prop
+      | .bool, t => nomatch t
+
+    namespace IsValue
+      theorem halts {τ: Ty} {t: Top τ}: IsValue τ t → Halts t := nomatch t
+    end IsValue
+
+    namespace Total
+      theorem halts {τ: Ty} {t: Top τ}: Top τ → Halts t
+        | t => nomatch t
+    end Total
+  end Top
+end Total.Stlc.Lang.Annotated
