Total/Stlc/Lang/Annotated/Theorems.lean
@@ -4,24 +4,57 @@ import Total.Relation
 import Total.Stlc.Lang.Annotated.Grammar
 import Total.Stlc.Lang.Annotated.Syntax
 import Total.Stlc.Lang.Annotated.Semantics
+import Total.Stlc.Lang.Annotated.Termination
+
+set_option autoImplicit false
 
 namespace Total.Stlc.Lang.Annotated
   namespace Ty
   end Ty
 
-  namespace Term
-      namespace Eval₁
-        theorem deterministic {ρ: Ty → Type} {τ: Ty} {t t₁ t₂: Term ρ τ}: Eval₁ ρ τ t t₁ → Eval₁ ρ τ t t₂ → t₁ = t₂ := sorry
-        theorem progress {ρ: Ty → Type} {τ: Ty} {t₁: Term ρ τ}: IsValue ρ τ t₁ ∨ ∃ t₂: Term ρ τ, Eval₁ ρ τ t₁ t₂ := sorry
+  namespace PrimOp
+    namespace Eval₁
+      theorem deterministic := sorry
+      theorem progress := sorry
 
-        -- TODO: Theorems for Strong Normalization
-      end Eval₁
+      theorem preservesHalting := sorry
+      theorem preservesTotality := sorry
+    end Eval₁
+  end PrimOp
+
+  namespace Term
+    namespace Eval₁
+      theorem deterministic {τ: Ty} {t t₁ t₂: Term τ}: Eval₁ τ t t₁ → Eval₁ τ t t₂ → t₁ = t₂ := sorry
+      theorem progress {τ: Ty} {t₁: Term τ}: IsValue τ t₁ ∨ ∃ t₂: Term τ, Eval₁ τ t₁ t₂ := sorry
+
+      theorem preservesHalting {τ: Ty} {t₁ t₂: Term τ} (he: Eval₁ τ t₁ t₂): Halts t₁ ↔ Halts t₂ := sorry
+      theorem preservesTotality {τ: Ty} {t₁ t₂: Term τ} (he: Eval₁ τ t₁ t₂): Total τ t₁ ↔ Total τ t₂ := sorry
+    end Eval₁
+
+    namespace Eval
+      theorem deterministic {τ: Ty} {t t₁ t₂: Term τ}: Eval₁ τ t t₁ → Eval₁ τ t t₂ → t₁ = t₂ := sorry
+      theorem progress {τ: Ty} {t₁: Term τ}: IsValue τ t₁ ∨ ∃ t₂: Term τ, Eval₁ τ t₁ t₂ := sorry
+
+      theorem preservesTotality {τ: Ty} {t₁ t₂: Term τ} (he: Eval τ t₁ t₂): Total τ t₁ ↔ Total τ t₂ := sorry
+      theorem normalization {τ: Ty} {t: Term τ}: Halts t := sorry
+    end Eval
   end Term
 
   namespace Top
-      namespace Eval₁
-        theorem deterministic {ρ: Ty → Type} {τ: Ty} {t t₁ t₂: Top ρ τ}: Eval₁ ρ τ t t₁ → Eval₁ ρ τ t t₂ → t₁ = t₂ := sorry
-        theorem progress {ρ: Ty → Type} {τ: Ty} {t₁: Top ρ τ}: IsValue ρ τ t₁ ∨ ∃ t₂: Top ρ τ, Eval₁ ρ τ t₁ t₂ := sorry
-      end Eval₁
+    namespace Eval₁
+      theorem deterministic {τ: Ty} {t t₁ t₂: Top ρ τ}: Eval₁ τ t t₁ → Eval₁ τ t t₂ → t₁ = t₂ := sorry
+      theorem progress {τ: Ty} {t₁: Top ρ τ}: IsValue τ t₁ ∨ ∃ t₂: Top ρ τ, Eval₁ τ t₁ t₂ := sorry
+
+      theorem preservesHalting {τ: Ty} {t₁ t₂: Top ρ τ} (he: Eval₁ τ t₁ t₂): Halts t₁ ↔ Halts t₂ := sorry
+      theorem preservesTotality {τ: Ty} {t₁ t₂: Top ρ τ} (he: Eval₁ τ t₁ t₂): Total τ t₁ ↔ Total τ t₂ := sorry
+    end Eval₁
+
+    namespace Eval
+      theorem deterministic {τ: Ty} {t t₁ t₂: Top ρ τ}: Eval₁ τ t t₁ → Eval₁ τ t t₂ → t₁ = t₂ := sorry
+      theorem progress {τ: Ty} {t₁: Top ρ τ}: IsValue τ t₁ ∨ ∃ t₂: Top ρ τ, Eval₁ τ t₁ t₂ := sorry
+
+      theorem preservesTotality {τ: Ty} {t₁ t₂: Top ρ τ} (he: Eval τ t₁ t₂): Total τ t₁ ↔ Total τ t₂ := sorry
+      theorem normalization {τ: Ty} {t: Top ρ τ}: Halts t := sorry
+    end Eval
   end Top
 end Total.Stlc.Lang.Annotated
