Total/Stlc/Lang/Surface/Termination.lean
@@ -1,0 +1,85 @@
+import Total.Relation
+
+import Total.Stlc.Lang.Surface.Grammar
+import Total.Stlc.Lang.Surface.Syntax
+import Total.Stlc.Lang.Surface.Semantics
+
+set_option autoImplicit false
+
+namespace Total.Stlc.Lang.Surface
+  namespace UnOp
+    @[reducible]
+    def Halts (op: UnOp) (t₁: Term): Prop := ∃ t₂: Term, Eval₁ op t₁ t₂ ∧ Term.IsValue t₂
+
+    @[reducible]
+    def Total (τ₁ τ₂: Ty) (op: UnOp) (t: Term): Prop :=
+      (HasType op τ₁ τ₂) ∧ (Halts op t) ∧ True
+
+    namespace Total
+      theorem halts {τ₁ τ₂: Ty} {op: UnOp} {t: Term}: Total τ₁ τ₂ op t → Halts op t
+        | ⟨_, hh, _⟩ => hh
+    end Total
+  end UnOp
+
+  namespace BinOp
+    @[reducible]
+    def Halts (op: BinOp) (t₁ t₂: Term): Prop := ∃ t₃: Term, Eval₁ op t₁ t₂ t₃ ∧ Term.IsValue t₃
+
+    @[reducible]
+    def Total (τ₁ τ₂ τ₃: Ty) (op: BinOp) (t₁ t₂: Term): Prop :=
+      (HasType op τ₁ τ₂ τ₃) ∧ (Halts op t₁ t₂) ∧ True
+
+    namespace Total
+      theorem halts {τ₁ τ₂ τ₃: Ty} {op: BinOp} {t₁ t₂: Term}: Total τ₁ τ₂ τ₃ op t₁ t₂ → Halts op t₁ t₂
+        | ⟨_, hh, _⟩ => hh
+    end Total
+  end BinOp
+
+  namespace Term
+    @[reducible]
+    def Halts (t₁: Term): Prop := ∃ t₂: Term, Eval t₁ t₂ ∧ IsValue t₂
+
+    @[reducible]
+    def Total (τ: Ty) (t: Term): Prop :=
+      (HasType t τ) ∧ (Halts t) ∧ (
+        match τ with
+          | .bool => True
+          | .nat  => True
+      )
+
+    namespace IsValue
+      theorem halts {t: Term}: IsValue t → Halts t
+        | .bool _ => ⟨_, .refl, .bool _⟩
+        | .nat  _ => ⟨_, .refl, .nat  _⟩
+    end IsValue
+
+    namespace Total
+      theorem halts {τ: Ty}: {t: Term} → Total τ t → Halts t
+        | .bool _, _ => IsValue.halts (.bool _)
+        | .nat _,  _ => IsValue.halts (.nat  _)
+
+        | .unOp _ _,    ⟨_, ⟨_, he, hv⟩, _⟩
+        | .binOp _ _ _, ⟨_, ⟨_, he, hv⟩, _⟩
+
+        | .cond _ _ _,  ⟨_, ⟨_, he, hv⟩, _⟩ => ⟨_, he, hv⟩
+    end Total
+  end Term
+
+  namespace Top
+    @[reducible]
+    def Halts (t₁: Top): Prop := ∃ t₂: Top, Eval t₁ t₂ ∧ IsValue t₂
+
+    @[reducible]
+    def Total: Ty → Top → Prop
+      | .bool, t => nomatch t
+
+    namespace IsValue
+      theorem halts {t: Top}: IsValue t → Halts t := nomatch t
+    end IsValue
+
+    namespace Total
+      theorem halts {τ: Ty} {t: Top}: Top → Halts t
+        | t => nomatch t
+    end Total
+  end Top
+end Total.Stlc.Lang.Surface
